James C - almost completed chapter 12 statics

isabelle/Chapter12_1_Language.thy
@@ -10,6 +10,14 @@ datatype type =
 | Void
 | Sum type type
 
+datatype patn =
+  WildPat
+| VarPat
+| TrivPat
+| PairPat patn patn
+| InLPat patn
+| InRPat patn
+
 datatype expr = 
   Var var
 | Zero
@@ -25,8 +33,21 @@ datatype expr =
 | Case expr expr expr
 | InL type type expr
 | InR type type expr
+| Match expr "rule list"
+and rule = 
+  Rule patn expr
+
+fun pat_var_count :: "patn => nat"
+where "pat_var_count WildPat = 0"
+    | "pat_var_count VarPat = 1"
+    | "pat_var_count TrivPat = 0"
+    | "pat_var_count (PairPat p1 p2) = pat_var_count p1 + pat_var_count p2"
+    | "pat_var_count (InLPat p) = pat_var_count p"
+    | "pat_var_count (InRPat p) = pat_var_count p"
 
 primrec insert :: "var => expr => expr"
+    and insert_rules :: "var => rule list => rule list"
+    and insert_rule :: "var => rule => rule"
 where "insert n (Var v) = Var (incr n v)"
     | "insert n Zero = Zero"
     | "insert n (Suc e) = Suc (insert n e)"
@@ -41,8 +62,18 @@ where "insert n (Var v) = Var (incr n v)"
     | "insert n (Case et el er) = Case (insert n et) (insert (next n) el) (insert (next n) er)"
     | "insert n (InL t1 t2 e) = InL t1 t2 (insert n e)"
     | "insert n (InR t1 t2 e) = InR t1 t2 (insert n e)"
+    | "insert n (Match e rs) = Match (insert n e) (insert_rules n rs)"
+    | "insert_rules n [] = []"
+    | "insert_rules n (r # rs) = insert_rule n r # insert_rules n rs"
+    | "insert_rule n (Rule p e) = Rule p (insert (next_by (pat_var_count p) n) e)"
+
+primrec mult_insert :: "nat => expr => expr"
+where "mult_insert 0 e = e"
+    | "mult_insert (Nat.Suc n) e = mult_insert n (insert first e)"
 
 primrec remove :: "var => expr => expr"
+    and remove_rules :: "var => rule list => rule list"
+    and remove_rule :: "var => rule => rule"
 where "remove n (Var v) = Var (subr n v)"
     | "remove n Zero = Zero"
     | "remove n (Suc e) = Suc (remove n e)"
@@ -57,8 +88,14 @@ where "remove n (Var v) = Var (subr n v)"
     | "remove n (Case et el er) = Case (remove n et) (remove (next n) el) (remove (next n) er)"
     | "remove n (InL t1 t2 e) = InL t1 t2 (remove n e)"
     | "remove n (InR t1 t2 e) = InR t1 t2 (remove n e)"
+    | "remove n (Match e rs) = Match (remove n e) (remove_rules n rs)"
+    | "remove_rules n [] = []"
+    | "remove_rules n (r # rs) = remove_rule n r # remove_rules n rs"
+    | "remove_rule n (Rule p e) = Rule p (remove (next_by (pat_var_count p) n) e)"
 
 primrec subst' :: "var => expr => expr => expr"
+    and subst_rules :: "var => expr => rule list => rule list"
+    and subst_rule :: "var => expr => rule => rule"
 where "subst' n e' (Var v) = (if v = n then e' else Var v)"
     | "subst' n e' Zero = Zero"
     | "subst' n e' (Suc e) = Suc (subst' n e' e)"
@@ -79,14 +116,28 @@ where "subst' n e' (Var v) = (if v = n then e' else Var v)"
                            (subst' (next n) (insert first e') er)"
     | "subst' n e' (InL t1 t2 e) = InL t1 t2 (subst' n e' e)"
     | "subst' n e' (InR t1 t2 e) = InR t1 t2 (subst' n e' e)"
+    | "subst' n e' (Match e rs) = Match (subst' n e' e) (subst_rules n e' rs)"
+    | "subst_rules n e' [] = []"
+    | "subst_rules n e' (r # rs) = subst_rule n e' r # subst_rules n e' rs"
+    | "subst_rule n e' (Rule p e) = Rule p (subst' (next_by (pat_var_count p) n) 
+                                                   (mult_insert (pat_var_count p) e') e)"
 
 definition subst :: "expr => expr => expr"
 where "subst e' e = remove first (subst' first (insert first e') e)"
 
 lemma [simp]: "remove n (insert n e) = e"
-by (induction e arbitrary: n, simp_all)
+  and [simp]: "remove_rules n (insert_rules n rs) = rs"
+  and [simp]: "remove_rule n (insert_rule n r) = r"
+by (induction e and rs and r arbitrary: n and n and n, simp_all)
 
 lemma [simp]: "canswap m n ==> insert m (insert n e) = insert (next n) (insert m e)"
-by (induction e arbitrary: n m, simp_all)
+  and [simp]: "canswap m n ==> 
+        insert_rules m (insert_rules n rs) = insert_rules (next n) (insert_rules m rs)"
+  and [simp]: "canswap m n ==> 
+        insert_rule m (insert_rule n r) = insert_rule (next n) (insert_rule m r)"
+by (induction e and rs and r arbitrary: n m and n m and n m, simp_all)
+
+lemma [simp]: "mult_insert m (insert n e) = insert (next_by m n) (mult_insert m e)"
+by (induction m arbitrary: n e, simp_all)
 
 end
