isabelle/Chapter12_2_Typechecking.thy
@@ -2,7 +2,25 @@ theory Chapter12_2_Typechecking
 imports Chapter12_1_Language
 begin
 
+inductive typecheck_patn :: "patn => type => type env => bool"
+where [simp]: "typecheck_patn VarPat t (extend empty_env t)"
+    | [simp]: "typecheck_patn WildPat t empty_env"
+    | [simp]: "typecheck_patn TrivPat Unit empty_env"
+    | [simp]: "typecheck_patn p1 t1 e1 ==> typecheck_patn p2 t2 e2 ==> 
+          typecheck_patn (PairPat p1 p2) (Prod t1 t2) (e1 +++ e2)"
+    | [simp]: "typecheck_patn p t e ==> typecheck_patn (InLPat p) (Sum t t2) e"
+    | [simp]: "typecheck_patn p t e ==> typecheck_patn (InRPat p) (Sum t2 t) e"
+
+inductive_cases [elim!]: "typecheck_patn VarPat t gam"
+inductive_cases [elim!]: "typecheck_patn WildPat t gam"
+inductive_cases [elim!]: "typecheck_patn TrivPat t gam"
+inductive_cases [elim!]: "typecheck_patn (PairPat p1 p2) t gam"
+inductive_cases [elim!]: "typecheck_patn (InLPat p) t gam"
+inductive_cases [elim!]: "typecheck_patn (InRPat p) t gam"
+
 inductive typecheck :: "type env => expr => type => bool"
+      and typecheck_rules :: "type env => type => rule list => type => bool"
+      and typecheck_rule :: "type env => type => rule => type => bool"
 where tc_var [simp]: "lookup gam x = Some t ==> typecheck gam (Var x) t"
     | tc_zero [simp]: "typecheck gam Zero Nat"
     | tc_suc [simp]: "typecheck gam e Nat ==> typecheck gam (Suc e) Nat"
@@ -21,6 +39,12 @@ where tc_var [simp]: "lookup gam x = Some t ==> typecheck gam (Var x) t"
                 typecheck (extend gam t2) er t ==> typecheck gam (Case et el er) t"
     | tc_inl [simp]: "typecheck gam e t1 ==> typecheck gam (InL t1 t2 e) (Sum t1 t2)"
     | tc_inr [simp]: "typecheck gam e t2 ==> typecheck gam (InR t1 t2 e) (Sum t1 t2)"
+    | tc_match [simp]: "typecheck gam (Match e rs) t"
+    | tc_rules_nil [simp]: "typecheck_rules gam t1 [] t"
+    | tc_rules_cons [simp]: "typecheck_rule gam t1 r t ==> typecheck_rules gam t1 rs t ==> 
+                typecheck_rules gam t1 (r # rs) t"
+    | tc_rule [simp]: "typecheck_patn p t1 gam1 ==> typecheck (gam1 +++ gam) e t ==>
+                typecheck_rule gam t1 (Rule p e) t"
 
 inductive_cases [elim!]: "typecheck gam (Var x) t"
 inductive_cases [elim!]: "typecheck gam Zero t"
@@ -36,14 +60,41 @@ inductive_cases [elim!]: "typecheck gam (Abort t1 e) t"
 inductive_cases [elim!]: "typecheck gam (Case et el er) t"
 inductive_cases [elim!]: "typecheck gam (InL t1 t2 e) t"
 inductive_cases [elim!]: "typecheck gam (InR t1 t2 e) t"
+inductive_cases [elim!]: "typecheck gam (Match e rs) t"
+inductive_cases [elim!]: "typecheck_rules gam t1 [] t"
+inductive_cases [elim!]: "typecheck_rules gam t1 (r # rs) t"
+inductive_cases [elim!]: "typecheck_rule gam t1 (Rule p e) t"
+
+lemma [simp]: "typecheck_patn p t gam ==> pat_var_count p = env_size gam"
+by (induction p t gam rule: typecheck_patn.induct, simp_all)
 
 lemma [simp]: "typecheck gam e t ==> n in gam ==> 
          typecheck (extend_at n gam t') (insert n e) t"
-by (induction gam e t arbitrary: n rule: typecheck.induct, fastforce+)
+  and [simp]: "typecheck_rules gam tt rs t ==> n in gam ==> 
+         typecheck_rules (extend_at n gam t') tt (insert_rules n rs) t"
+  and [simp]: "typecheck_rule gam tt r t ==> n in gam ==> 
+         typecheck_rule (extend_at n gam t') tt (insert_rule n r) t"
+proof (induction gam e t and gam tt rs t and gam tt r t arbitrary: n and n and n 
+       rule: typecheck_typecheck_rules_typecheck_rule.inducts, fastforce+)
+case (tc_rule p t1 gam1 gam e t)
+  hence "(next_by (env_size gam1) n) in (gam1 +++ gam)" by simp
+  with tc_rule show ?case by fastforce
+qed 
+
+lemma [simp]: "typecheck gam e t ==> typecheck (gam1 +++ gam) (mult_insert (env_size gam1) e) t"
+by simp 
+sorry
 
 lemma [simp]: "typecheck (extend_at n gam t') e t ==> n in gam ==> typecheck gam e' t' ==> 
         typecheck gam (remove n (subst' n (insert n e') e)) t"
-by (induction "extend_at n gam t'" e t arbitrary: n gam t' e' rule: typecheck.induct, fastforce+)
+  and [simp]: "typecheck_rules (extend_at n gam t') tt rs t ==> n in gam ==> typecheck gam e' t' ==> 
+        typecheck_rules  gam tt (remove_rules n (subst_rules n (insert n e') rs)) t"
+  and [simp]: "typecheck_rule (extend_at n gam t') tt r t ==> n in gam ==> typecheck gam e' t' ==> 
+        typecheck_rule gam tt (remove_rule n (subst_rule n (insert n e') r)) t"
+by (induction "extend_at n gam t'" e t and "extend_at n gam t'" tt rs t 
+          and "extend_at n gam t'" tt r t 
+    arbitrary: n gam t' e' and n gam t' e' and n gam t' e'
+    rule: typecheck_typecheck_rules_typecheck_rule.inducts, fastforce+)
 
 lemma [simp]: "typecheck (extend gam t') e t ==> typecheck gam e' t' ==> 
                           typecheck gam (subst e' e) t"
